mergeable_states from partial_state
Redefine mergeable_states so that a pair of partial states is mergeable
if they can be generated as partializations of a complete state that
originates from an initial state after a sequence of steps. We want to
know enough about the pairs of states that are mergeable to allow
meaningful reasoning, and this view corresponds to the more restricted
scenarios that are envisioned.

The change requires some substantial changes to existing composition
proofs; many of these are amended presently. Some auxiliary lemmas and
invariants may still be missing.

Intermediate/PS.v
@@ -363,13 +363,22 @@ Proof.
   - apply (closed_interface_sym _ _ Hclosed).
 Qed.
 
-(* NOTE: Instance of a more general property which may be added to CoqUtils. *)
+(* NOTE: Instance of a more general property which may be added to CoqUtils.
+   TODO: Harmonize naming of two directions or unify with iff. *)
 Lemma domm_partition :
   forall ctx1 ctx2,
     mergeable_interfaces ctx1 ctx2 ->
   forall C,
     C \notin domm ctx2 ->
     C \in domm ctx1.
+Admitted. (* Rank 1. *)
+
+Lemma domm_partition_notin :
+  forall ctx1 ctx2,
+    mergeable_interfaces ctx1 ctx2 ->
+  forall C,
+    C \in domm ctx2 ->
+    C \notin domm ctx1.
 Admitted. (* Rank 1. *)
 
 Inductive mergeable_states_pc_cc: state -> state -> Prop :=
@@ -379,23 +388,11 @@ Inductive mergeable_states_pc_cc: state -> state -> Prop :=
     mergeable_states_pc_cc (CC (C1, gps1, mem1)) (PC (gps2, mem2, regs2, pc2)).
 
 Inductive mergeable_states (ctx1 ctx2: Program.interface): state -> state -> Prop :=
-| mergeable_states_first: forall ips1 ips2,
+| mergeable_states_intro: forall ics ips1 ips2,
     mergeable_interfaces ctx1 ctx2 ->
-    is_program_component ips1 ctx1 ->
-    is_context_component ips2 ctx2 ->
-    mergeable_states_pc_cc ips1 ips2 ->
-    state_component ips1 = state_component ips2 ->
-    mergeable_stacks (state_stack ips1) (state_stack ips2) ->
-    mergeable_memories (state_memory ips1) (state_memory ips2) ->
-    mergeable_states ctx1 ctx2 ips1 ips2
-| mergeable_states_second: forall ips1 ips2,
-    mergeable_interfaces ctx1 ctx2 ->
-    is_context_component ips1 ctx1 ->
-    is_program_component ips2 ctx2 ->
-    mergeable_states_pc_cc ips1 ips2 ->
-    state_component ips1 = state_component ips2 ->
-    mergeable_stacks (state_stack ips1) (state_stack ips2) ->
-    mergeable_memories (state_memory ips1) (state_memory ips2) ->
+    CS.comes_from_initial_state ics ->
+    partial_state ctx1 ics ips1 ->
+    partial_state ctx2 ics ips2 ->
     mergeable_states ctx1 ctx2 ips1 ips2.
 
 Lemma mergeable_stack_frames_sym:
@@ -418,6 +415,12 @@ Proof.
     constructor; auto.
   - apply mergeable_stack_frames_sym; auto.
 Qed.
+
+Lemma mergeable_stacks_partition gps ctx1 ctx2:
+  mergeable_interfaces ctx1 ctx2 ->
+  mergeable_stacks (to_partial_stack gps (domm ctx1)) (to_partial_stack gps (domm ctx2)).
+Proof.
+Admitted. (* Grade 2. *)
 
 Lemma mergeable_memories_sym:
   forall pmem1 pmem2,
@@ -449,16 +452,24 @@ Lemma mergeable_states_sym:
 Proof.
   intros p c s1 s2 Hp_wf Hc_wf Hlink Hmergeable.
   inversion Hmergeable; subst.
-  - apply mergeable_states_second; auto.
+  - econstructor; auto.
     + apply mergeable_interfaces_sym; assumption.
-    + apply mergeable_states_pc_cc_sym; assumption.
-    + apply mergeable_stacks_sym; assumption.
-    + apply mergeable_memories_sym; assumption.
-  - apply mergeable_states_first; auto.
-    + apply mergeable_interfaces_sym; assumption.
-    + apply mergeable_states_pc_cc_sym; assumption.
-    + apply mergeable_stacks_sym; assumption.
-    + apply mergeable_memories_sym; assumption.
+    + eassumption.
+    + eassumption.
+    + eassumption.
+Qed.
+
+Lemma mergeable_states_stacks ctx1 ctx2 ips1 ips2 gps1 gps2:
+  mergeable_states ctx1 ctx2 ips1 ips2 ->
+  state_stack ips1 = gps1 ->
+  state_stack ips2 = gps2 ->
+  mergeable_stacks gps1 gps2.
+Proof.
+  intros Hmerge Hstk1 Hstk2.
+  inversion Hmerge as [ics ? ? Hmerge_ifaces Hprovenance Hpartial1 Hpartial2]; subst.
+    inversion Hpartial1; subst;
+    inversion Hpartial2; subst;
+    apply mergeable_stacks_partition; assumption.
 Qed.
 
 Definition merge_stack_frames (frames: PartialPointer.t * PartialPointer.t): PartialPointer.t :=
